WIP

PerformanceExperiments/csv_to_txt.py
@@ -25,16 +25,18 @@ def split_to_kinds(data):
     for kind, rows in rows_by_kind.items():
         headings = sorted(set(k for row in rows for k, v in row.items() if k != 'param kind' and v is not None and v != ''))
         headings = [k for k in headings if k.startswith('param ')] + [k for k in headings if not k.startswith('param ')]
+        headings = [k for k in headings if 'user' not in k and 'sys' not in k] # TEMP
         for k in headings:
             if any(row[k] is None or row[k] == '' for row in rows):
-                print('Warning: Mix of empty and non-empty entries for key %s in kind %s:\n%s' % (k, kind, repr([row[k] for row in rows])), file=sys.stderr)
+                # print('Warning: Mix of empty and non-empty entries for key %s in kind %s:\n%s' % (k, kind, repr([row[k] for row in rows])), file=sys.stderr)
+                pass
         ret[kind] = ([tuple(k.replace(' ', '-').replace('_', '-') for k in headings)] +
                      [tuple(row[k] for k in headings) for row in rows])
     return ret
 
 def emit_output(kind, rows):
     with open('%s.txt' % kind.replace('_', '-').replace(' ', '-'), 'w') as f:
-        f.write('\n'.join(map(' '.join, rows)))
+        f.write('\n'.join(','.join(v.replace(',', '-') for v in row) for row in rows))
 
 if __name__ == '__main__':
     args = parser.parse_args()
